Correctly handle integer promotions and usual arithmetic conventions.
Other minor changes:
* Split the various kinds of operations. This allows us to type these correctly.
* Allow casts from a type to itself
* Insert casts before assignments (in the semantics)
* Insert casts before function calls (in the frontend, function calls are
  untyped in the expression semantics, so we cannot do that in the semantics)

abstract_integers.v
@@ -18,42 +18,38 @@ Local Open Scope Z_scope.
 (** * Syntax of integer operations *)
 (** The inductive types [unop] and [binop] describe the abstract syntax of the
 C integer operations. *)
-Inductive comp_kind := CEq | CLt | CLe.
-Inductive unop := NegOp | ComplOp.
-Inductive bitop := BAnd | BOr | BXor.
+Inductive compop := EqOp | LtOp | LeOp.
+Inductive bitop := AndOp | OrOp | XorOp.
+Inductive arithop := PlusOp | MinusOp | MultOp | DivOp | ModOp.
+Inductive shiftop := ShiftLOp | ShiftROp.
 Inductive binop :=
-  | PlusOp | MinusOp | MultOp | ShiftLOp | ShiftROp | DivOp | ModOp
-  | CompOp : comp_kind → binop | BitOp : bitop → binop.
-Notation EqOp := (CompOp CEq).
-Notation LtOp := (CompOp CLt).
-Notation LeOp := (CompOp CLe).
-Notation AndOp := (BitOp BAnd).
-Notation OrOp := (BitOp BOr).
-Notation XorOp := (BitOp BXor).
+  | CompOp : compop → binop
+  | ArithOp : arithop → binop
+  | ShiftOp : shiftop → binop
+  | BitOp : bitop → binop.
+Inductive unop := NegOp | ComplOp | NotOp.
 
-Instance unop_dec (op1 op2 : unop) : Decision (op1 = op2).
-Proof. solve_decision. Defined.
-Instance comp_kind_dec (c1 c2 : comp_kind) : Decision (c1 = c2).
+Instance comp_kind_dec (op1 op2 : compop) : Decision (op1 = op2).
 Proof. solve_decision. Defined.
 Instance bitop_dec (op1 op2 : bitop) : Decision (op1 = op2).
 Proof. solve_decision. Defined.
+Instance arithop_dec (op1 op2 : arithop) : Decision (op1 = op2).
+Proof. solve_decision. Defined.
+Instance shiftop_dec (op1 op2 : shiftop) : Decision (op1 = op2).
+Proof. solve_decision. Defined.
 Instance binop_dec (op1 op2 : binop) : Decision (op1 = op2).
 Proof. solve_decision. Defined.
+Instance unop_dec (op1 op2 : unop) : Decision (op1 = op2).
+Proof. solve_decision. Defined.
 
-Definition Z_comp (c : comp_kind) : Z → Z → Prop :=
-  match c with CEq => (=) | CLt => (<) | CLe => (≤) end.
+Definition Z_comp (c : compop) : Z → Z → Prop :=
+  match c with EqOp => (=) | LtOp => (<) | LeOp => (≤) end.
 Instance Z_comp_dec c : ∀ x y, Decision (Z_comp c x y) :=
   match c return ∀ x y : Z, Decision (Z_comp c x y) with
-  | CEq => decide_rel (=) | CLt => decide_rel (<) | CLe => decide_rel (≤)
-  end.
-Definition nat_comp (c : comp_kind) : nat → nat → Prop :=
-  match c with CEq => (=) | CLt => (<) | CLe => (≤) end.
-Instance nat_comp_dec c : ∀ x y, Decision (nat_comp c x y) :=
-  match c return ∀ x y : nat, Decision (nat_comp c x y) with
-  | CEq => decide_rel (=) | CLt => decide_rel (<) | CLe => decide_rel (≤)
+  | EqOp => decide_rel (=) | LtOp => decide_rel (<) | LeOp => decide_rel (≤)
   end.
 Definition bool_bitop (op : bitop) : bool → bool → bool :=
-  match op with BAnd => (&&) | BOr => (||) | BXor => xorb end.
+  match op with AndOp => (&&) | OrOp => (||) | XorOp => xorb end.
 
 (** * Operations on machine integers *)
 (** The abstract interface for machine integers is parametrized by a type [Ti]
@@ -64,13 +60,13 @@ Inductive signedness := Signed | Unsigned.
 Instance signedness_eq_dec (s1 s2 : signedness) : Decision (s1 = s2).
 Proof. solve_decision. Defined.
 
-Inductive int_type (Ti : Set) := IntType { ISign : signedness; IRank : Ti }.
+Inductive int_type (Ti : Set) := IntType { sign : signedness; rank : Ti }.
 Add Printing Constructor int_type.
 Delimit Scope int_type_scope with IT.
 Bind Scope int_type_scope with int_type.
 Arguments IntType {_} _ _.
-Arguments ISign {_} _%IT.
-Arguments IRank {_} _%IT.
+Arguments sign {_} _%IT.
+Arguments rank {_} _%IT.
 
 Instance int_type_eq_dec {Ti : Set} `{∀ k1 k2 : Ti, Decision (k1 = k2)}
   (τ1 τ2 : int_type Ti) : Decision (τ1 = τ2).
@@ -108,6 +104,7 @@ Arguments char_bits _ _ : simpl never.
 Arguments rank_size _ _ _ : simpl never.
 Arguments endianize _ _ _ _ : simpl never.
 Arguments deendianize _ _ _ _ : simpl never.
+Arguments int_rank_eq_dec _ _ _ _ : simpl never.
 
 Notation "'ucharT'" := (IntType Unsigned char_rank) : int_type_scope.
 Notation "'scharT'" := (IntType Signed char_rank) : int_type_scope.
@@ -116,47 +113,19 @@ Notation "'sintT'" := (IntType Signed int_rank) : int_type_scope.
 Notation "'uptrT'" := (IntType Unsigned ptr_rank) : int_type_scope.
 Notation "'sptrT'" := (IntType Signed ptr_rank) : int_type_scope.
 
-(** The class [IntEnv] extends the previously defined class with binary integer
-operations and casts. Unary operations are derived from the binary operations,
-and integer promotions/demotions are handled explicitly using casts. *)
-
-(** In order to deal with underspecification of operations, the class [IntEnv]
-does not just contain a function [int_binop] to perform a binary operation, but
-also a predicate [int_binop_ok τ op x y] that describes when [op] is allowed to
-be performed on integers [x] and [y] of type [τ]. This is to allow both strict
-implementations that make integer overflow undefined, and those that let it
-wrap (as for example GCC with the -fno-strict-overflow flag does). When an
-operation is allowed by the C standard, the result of [int_binop τ op x y]
-should correspond to its specification by the standard. *)
-Class IntEnv (Ti : Set) := {
-  int_coding :>> IntCoding Ti;
-  int_binop_ok : int_type Ti → binop → Z → Z → Prop;
-  int_binop : int_type Ti → binop → Z → Z → Z;
-  int_cast_ok : int_type Ti → Z → Prop;
-  int_cast : int_type Ti → Z → Z;
-  int_binop_ok_dec τ op x y :> Decision (int_binop_ok τ op x y);
-  int_cast_ok_dec τ x :> Decision (int_cast_ok τ x)
-}.
-
-Arguments int_binop_ok _ _ _ _ _ _ : simpl never.
-Arguments int_binop _ _ _ _ _ _ : simpl never.
-Arguments int_cast_ok _ _ _ _ : simpl never.
-Arguments int_cast _ _ _ _ : simpl never.
-
 (** * The abstract interface for machine integers *)
 (** In order to declare classes to describe the laws of an implementation of
 machine integers, we first define functions to encode and decode integers, and
 functions to relate binary operations and casts to its specification. *)
-Section least_operations.
+Section int_coding.
   Context `{IntCoding Ti}.
 
-  Definition int_size (τ : int_type Ti) : nat := rank_size (IRank τ).
-  Global Arguments int_size !_ /.
-  Definition int_bits (τ : int_type Ti) : nat := (int_size τ * char_bits)%nat.
+  Definition int_bits (τ : int_type Ti) : nat :=
+    (rank_size (rank τ) * char_bits)%nat.
   Definition int_lower (τ : int_type Ti) : Z :=
-    match ISign τ with Signed => -2 ^ (int_bits τ - 1) | Unsigned => 0 end.
+    match sign τ with Signed => -2 ^ (int_bits τ - 1) | Unsigned => 0 end.
   Definition int_upper (τ : int_type Ti) : Z :=
-    match ISign τ with
+    match sign τ with
     | Signed => 2 ^ (int_bits τ - 1) | Unsigned => 2 ^ int_bits τ
     end.
   Definition int_typed (x : Z) (τ : int_type Ti) : Prop :=
@@ -170,114 +139,166 @@ Section least_operations.
     match bs with [] => 0 | b :: bs => Z.b2z b + 2 * Z_of_bits bs end.
 
   Definition int_to_bits (τ : int_type Ti) (x : Z) : list bool :=
-    endianize (IRank τ) $ Z_to_bits (int_bits τ) $
-      match ISign τ with
+    endianize (rank τ) $ Z_to_bits (int_bits τ) $
+      match sign τ with
       | Signed => if decide (0 ≤ x) then x else x + 2 ^ int_bits τ
       | Unsigned => x
       end.
   Definition int_of_bits (τ : int_type Ti) (bs : list bool) : Z :=
-    let x := Z_of_bits (deendianize (IRank τ) bs) in
-    match ISign τ with
+    let x := Z_of_bits (deendianize (rank τ) bs) in
+    match sign τ with
     | Signed =>
        if decide (2 * x < 2 ^ int_bits τ) then x else x - 2 ^ int_bits τ
     | Unsigned => x
     end.
 
-  Definition int_binop_ok_ (τ : int_type Ti)
-      (op : binop) (x y : Z) : Prop :=
-    match op, ISign τ with
+  Definition int_pre_arithop_ok
+      (op : arithop) (x y : Z) (τ : int_type Ti) : Prop :=
+    match op, sign τ with
     | PlusOp, Signed => int_lower τ ≤ x + y < int_upper τ
     | PlusOp, Unsigned => True
     | MinusOp, Signed => int_lower τ ≤ x - y < int_upper τ
     | MinusOp, Unsigned => True
     | MultOp, Signed => int_lower τ ≤ x * y < int_upper τ
     | MultOp, Unsigned => True
-    | ShiftLOp, Signed => 0 ≤ x ∧ 0 ≤ y < int_bits τ ∧ x ≪ y < int_upper τ
-    | ShiftLOp, Unsigned => y < int_bits τ
-    | ShiftROp, Signed => 0 ≤ x ∧ 0 ≤ y < int_bits τ
-    | ShiftROp, Unsigned => y < int_bits τ
       (* Can still overflow, e.g. [-10 `quot` -1 = 10]. Maybe a tighter
          condition is possible. *)
     | DivOp, Signed => y ≠ 0 ∧ int_lower τ ≤ x `quot` y < int_upper τ
     | DivOp, Unsigned => y ≠ 0
     | ModOp, _ => y ≠ 0
-    | CompOp c, _ => True
-    | BitOp _, _ => True
     end.
-  Definition int_binop_ (τ : int_type Ti) (op : binop) (x y : Z) : Z :=
-    match op, ISign τ with
+  Definition int_pre_arithop (op : arithop) (x y : Z) (τ : int_type Ti) : Z :=
+    match op, sign τ with
     | PlusOp, Signed => x + y
     | PlusOp, Unsigned => (x + y) `mod` int_upper τ
     | MinusOp, Signed => x - y
     | MinusOp, Unsigned => (x - y) `mod` int_upper τ
     | MultOp, Signed => x * y
     | MultOp, Unsigned => (x * y) `mod` int_upper τ
+    | DivOp, _ => x `quot` y
+    | ModOp, _ => x `rem` y
+    end.
+  Definition int_pre_shiftop_ok
+      (op : shiftop) (x y : Z) (τ : int_type Ti) : Prop :=
+    match op, sign τ with
+    | ShiftLOp, Signed => 0 ≤ x ∧ 0 ≤ y < int_bits τ ∧ x ≪ y < int_upper τ
+    | ShiftLOp, Unsigned => 0 ≤ y < int_bits τ
+    | ShiftROp, Signed => 0 ≤ x ∧ 0 ≤ y < int_bits τ
+    | ShiftROp, Unsigned => 0 ≤ y < int_bits τ
+    end.
+  Definition int_pre_shiftop (op : shiftop) (x y : Z) (τ : int_type Ti) : Z :=
+    match op, sign τ with
     | ShiftLOp, Signed => x ≪ y
     | ShiftLOp, Unsigned => (x ≪ y) `mod` int_upper τ
     | ShiftROp, _ => x ≫ y
-    | DivOp, _ => x `quot` y
-    | ModOp, _ => x `rem` y
-    | CompOp c, _ => Z_of_sumbool (decide_rel (Z_comp c) x y)
-    | BitOp op, _ => int_of_bits τ (zip_with (bool_bitop op)
-        (int_to_bits τ x) (int_to_bits τ y))
     end.
-
-  Definition int_cast_ok_ (σ : int_type Ti) (x : Z) :=
-    match ISign σ with
-    | Signed => int_lower σ ≤ x < int_upper σ | Unsigned => True
+  Definition int_pre_cast_ok (σ : int_type Ti) (x : Z) :=
+    match sign σ with
+    | Signed =>
+       (**i actually implementation defined, see 6.3.1.3 *)
+       int_lower σ ≤ x < int_upper σ
+    | Unsigned => True
     end.
-  Definition int_cast_ (σ : int_type Ti) (x : Z) :=
-    match ISign σ with Signed => x | Unsigned => x `mod` int_upper σ end.
+  Definition int_pre_cast (σ : int_type Ti) (x : Z) :=
+    match sign σ with Signed => x | Unsigned => x `mod` int_upper σ end.
 
-  Global Instance int_binop_ok_dec_ τ op x y :
-    Decision (int_binop_ok_ τ op x y).
-  Proof. unfold int_binop_ok_. destruct op, (ISign τ); apply _. Defined.
-  Global Instance int_cast_ok_dec_ σ x : Decision (int_cast_ok_ σ x).
-  Proof. unfold int_cast_ok_. destruct (ISign σ); apply _. Defined.
-End least_operations.
+  Global Instance int_pre_arithop_ok_dec op x y τ :
+    Decision (int_pre_arithop_ok op x y τ).
+  Proof. unfold int_pre_arithop_ok. destruct op, (sign τ); apply _. Defined.
+  Global Instance int_pre_shiftop_ok_dec op x y τ :
+    Decision (int_pre_shiftop_ok op x y τ).
+  Proof. unfold int_pre_shiftop_ok. destruct op, (sign τ); apply _. Defined.
+  Global Instance int_pre_cast_ok_dec σ x : Decision (int_pre_cast_ok σ x).
+  Proof. unfold int_pre_cast_ok. destruct (sign σ); apply _. Defined.
 
-Section operations.
-  Context `{IntEnv Ti}.
+  Definition int_promote (τ : int_type Ti) : int_type Ti :=
+    if decide (rank_size (rank τ) < rank_size int_rank) then sintT%IT
+    else if decide (rank_size (rank τ) = rank_size int_rank)
+      then IntType (sign τ) int_rank
+    else τ.
+  Global Instance int_union : Union (int_type Ti) := λ τ1 τ2,
+    if decide (sign τ1 = sign τ2)
+      then if decide (rank_size (rank τ1) ≤ rank_size (rank τ2)) then τ2 else τ1
+    else if decide (sign τ1 = Unsigned
+      ∧ rank_size (rank τ2) ≤ rank_size (rank τ1)) then τ1
+    else if decide (sign τ2 = Unsigned
+      ∧ rank_size (rank τ1) ≤ rank_size (rank τ2)) then τ2
+    else if decide (sign τ1 = Signed
+      ∧ rank_size (rank τ2) < rank_size (rank τ1)) then τ1 else τ2.
+End int_coding.
 
-  Definition int_unop_ok (τ : int_type Ti) (op : unop) (x : Z) : Prop :=
-    match op with NegOp => int_binop_ok τ MinusOp 0 x | ComplOp => True end.
-  Global Instance int_unop_ok_dec τ op x : Decision (int_unop_ok τ op x).
-  Proof. destruct op; apply _. Defined.
-  Definition int_unop (τ : int_type Ti) (op : unop) (x : Z) : Z :=
-    match op with
-    | NegOp => int_binop τ MinusOp 0 x
-    | ComplOp => int_of_bits τ (negb <$> int_to_bits τ x)
-    end.
-End operations.
-
-(** The classes [IntCodingSpec] and [IntEnvSpec] describe the laws that an
-implementation of machine integers should satisfy. Most of these laws are
-straightforward. *)
+(** The classes [IntCodingSpec] describe the laws that an implementation of
+machine integers should satisfy with respect to representatons. *)
 Class IntCodingSpec Ti `{IntCoding Ti} := {
   char_bits_ge_8 : (8 ≤ char_bits)%nat;
   rank_size_char : rank_size char_rank = 1%nat;
   rank_size_pos k : (0 < rank_size k)%nat;
-
+  rank_size_injective :> Injective (=) (=) rank_size;
   endianize_permutation τ bs : endianize τ bs ≡ₚ bs;
   deendianize_endianize τ bs : deendianize τ (endianize τ bs) = bs;
   endianize_deendianize τ bs : endianize τ (deendianize τ bs) = bs
 }.
 
+(** In order to deal with underspecification of operations, the class [IntEnv]
+does not just contain a function [int_binop] to perform a binary operation, but
+also a predicate [int_binop_ok τ op x y] that describes when [op] is allowed to
+be performed on integers [x] and [y] of type [τ]. This is to allow both strict
+implementations that make integer overflow undefined, and those that let it
+wrap (as for example GCC with the -fno-strict-overflow flag does). When an
+operation is allowed by the C standard, the result of [int_binop τ op x y]
+should correspond to its specification by the standard. *)
+Class IntEnv (Ti : Set) := {
+  int_coding :>> IntCoding Ti;
+  int_arithop_ok : arithop → Z → int_type Ti → Z → int_type Ti → Prop;
+  int_arithop : arithop → Z → int_type Ti → Z → int_type Ti → Z;
+  int_shiftop_ok : shiftop → Z → int_type Ti → Z → int_type Ti → Prop;
+  int_shiftop : shiftop → Z → int_type Ti → Z → int_type Ti → Z;
+  int_cast_ok : int_type Ti → Z → Prop;
+  int_cast : int_type Ti → Z → Z;
+  int_arithop_ok_dec op x τ1 y τ2 :> Decision (int_arithop_ok op x τ1 y τ2);
+  int_shiftop_ok_dec op x τ1 y τ2 :> Decision (int_shiftop_ok op x τ1 y τ2);
+  int_cast_ok_dec σ x :> Decision (int_cast_ok σ x)
+}.
+Arguments int_arithop_ok _ _ _ _ _ _ _ : simpl never.
+Arguments int_arithop _ _ _ _ _ _ _ : simpl never.
+Arguments int_shiftop_ok _ _ _ _ _ _ _ : simpl never.
+Arguments int_shiftop _ _ _ _ _ _ _ : simpl never.
+Arguments int_cast_ok _ _ _ _ : simpl never.
+Arguments int_cast _ _ _ _ : simpl never.
+
 Class IntEnvSpec Ti `{IntEnv Ti} := {
   int_coding_spec :>> IntCodingSpec Ti;
-
-  int_binop_ok_more τ op x y :
-    int_binop_ok_ τ op x y → int_binop_ok τ op x y;
-  int_binop_ok_typed τ op x y :
-    int_typed x τ → int_typed y τ →
-    int_binop_ok τ op x y → int_typed (int_binop τ op x y) τ;
-  int_binop_spec τ op x y :
-    int_typed x τ → int_typed y τ → int_binop_ok_ τ op x y →
-    int_binop τ op x y = int_binop_ τ op x y;
-
-  int_cast_ok_more σ x : int_cast_ok_ σ x → int_cast_ok σ x;
-  int_cast_ok_typed σ x : int_cast_ok σ x → int_typed (int_cast σ x) σ;
-  int_cast_spec σ x : int_cast_ok_ σ x → int_cast σ x = int_cast_ σ x
+  int_arithop_ok_more op x y τ1 τ2 :
+    int_typed x τ1 → int_typed y τ2 →
+    let τ' := int_promote τ1 ∪ int_promote τ2 in
+    int_pre_arithop_ok op (int_pre_cast τ' x) (int_pre_cast τ' y) τ' →
+    int_arithop_ok op x τ1 y τ2;
+  int_arithop_typed op x y τ1 τ2 :
+    int_typed x τ1 → int_typed y τ2 →
+    int_arithop_ok op x τ1 y τ2 →
+    int_typed (int_arithop op x τ1 y τ2) (int_promote τ1 ∪ int_promote τ2);
+  int_arithop_spec op x y τ1 τ2 :
+    int_typed x τ1 → int_typed y τ2 →
+    let τ' := int_promote τ1 ∪ int_promote τ2 in
+    int_pre_arithop_ok op (int_pre_cast τ' x) (int_pre_cast τ' y) τ' →
+    int_arithop op x τ1 y τ2
+    = int_pre_arithop op (int_pre_cast τ' x) (int_pre_cast τ' y) τ';
+  int_shiftop_ok_more op x y τ1 τ2 :
+    int_typed x τ1 → int_typed y τ2 →
+    let τ' := int_promote τ1 in
+    int_pre_shiftop_ok op (int_pre_cast τ' x) y τ' →
+    int_shiftop_ok op x τ1 y τ2;
+  int_shiftop_typed op x y τ1 τ2 :
+    int_typed x τ1 → int_typed y τ2 → int_shiftop_ok op x τ1 y τ2 →
+    int_typed (int_shiftop op x τ1 y τ2) (int_promote τ1);
+  int_shiftop_spec op x y τ1 τ2 :
+    int_typed x τ1 → int_typed y τ2 →
+    let τ' := int_promote τ1 in
+    int_pre_shiftop_ok op x y τ' →
+    int_shiftop op x τ1 y τ2 = int_pre_shiftop op x y τ';
+  int_cast_ok_more σ x : int_pre_cast_ok σ x → int_cast_ok σ x;
+  int_cast_typed σ x : int_cast_ok σ x → int_typed (int_cast σ x) σ;
+  int_cast_spec σ x : int_pre_cast_ok σ x → int_cast σ x = int_pre_cast σ x
 }.
 
 (** * Theorems *)
@@ -310,7 +331,7 @@ Qed.
 Lemma Z_of_zero_bits n : Z_of_bits (replicate n false) = 0.
 Proof. induction n; simpl; lia. Qed.
 
-Section int_coding.
+Section properties.
 Context `{IntCodingSpec Ti}.
 Implicit Types τ : int_type Ti.
 Implicit Types k : Ti.
@@ -334,19 +355,10 @@ Proof. by rewrite endianize_permutation. Qed.
 Lemma deendianize_length k bs : length (deendianize k bs) = length bs.
 Proof. by rewrite deendianize_permutation. Qed.
 
-Lemma int_size_pos τ : (0 < int_size τ)%nat.
-Proof. apply rank_size_pos. Qed.
-Lemma int_size_ne_0 τ : (int_size τ ≠ 0)%nat.
+Lemma rank_size_ne_0 k : (rank_size k ≠ 0)%nat.
 Proof. apply Nat.neq_0_lt_0, rank_size_pos. Qed.
-Lemma int_size_pos_alt τ : 0 < int_size τ.
-Proof. apply (Nat2Z.inj_lt 0), rank_size_pos. Qed.
-
-Lemma int_size_char si : int_size (IntType si char_rank) = 1%nat.
-Proof. apply rank_size_char. Qed.
 Lemma int_bits_char si : int_bits (IntType si char_rank) = char_bits.
-Proof.
-  unfold int_bits, int_size; simpl. by rewrite rank_size_char, Nat.mul_1_l.
-Qed.
+Proof. unfold int_bits; simpl. by rewrite rank_size_char, Nat.mul_1_l. Qed.
 Lemma char_bits_pos : (0 < char_bits)%nat.
 Proof. pose proof char_bits_ge_8; lia. Qed.
 Lemma char_bits_ne_0 : char_bits ≠ 0%nat.
@@ -355,7 +367,7 @@ Lemma int_bits_ge_8 τ : (8 ≤ int_bits τ)%nat.
 Proof.
   unfold int_bits. transitivity (1 * char_bits)%nat.
   * by rewrite char_bits_ge_8, Nat.mul_1_l.
-  * apply Nat.mul_le_mono_r. generalize (int_size_pos τ); lia.
+  * apply Nat.mul_le_mono_r. generalize (rank_size_pos (rank τ)); lia.
 Qed.
 Lemma int_bits_ge_8_alt τ : 8 ≤ int_bits τ.
 Proof. apply (Nat2Z.inj_le 8), int_bits_ge_8. Qed.
@@ -363,27 +375,23 @@ Lemma int_bits_pos τ : (0 < int_bits τ)%nat.
 Proof. pose proof (int_bits_ge_8 τ); lia. Qed.
 Lemma int_bits_pos_alt τ : 0 < int_bits τ.
 Proof. apply (Nat2Z.inj_lt 0), int_bits_pos. Qed.
-
 Lemma int_bits_pred_nonneg τ : 0 ≤ int_bits τ - 1.
 Proof. pose proof (int_bits_pos_alt τ); lia. Qed.
 Hint Resolve int_bits_pos_alt int_bits_pred_nonneg.
-
 Lemma int_typed_lower x τ : int_typed x τ → int_lower τ ≤ x.
 Proof. by intros [??]. Qed.
 Lemma int_typed_upper x τ : int_typed x τ → x < int_upper τ.
 Proof. by intros [??]. Qed.
-
-Lemma int_lower_u τ : ISign τ = Unsigned → int_lower τ = 0.
+Lemma int_lower_u τ : sign τ = Unsigned → int_lower τ = 0.
 Proof. by destruct τ as [[]?]. Qed.
 Lemma int_lower_nonpos τ : int_lower τ ≤ 0.
 Proof.
-  unfold int_lower. destruct (ISign τ); [|done].
+  unfold int_lower. destruct (sign τ); [|done].
   apply Z.opp_nonpos_nonneg; auto with zpos.
 Qed.
 Lemma int_upper_pos τ : 0 < int_upper τ.
-Proof. unfold int_upper. destruct (ISign τ); auto with zpos. Qed.
+Proof. unfold int_upper. destruct (sign τ); auto with zpos. Qed.
 Hint Resolve int_lower_nonpos int_upper_pos.
-
 Lemma int_mod_lower_upper x τ :
   int_lower τ ≤ x `mod` int_upper τ < int_upper τ.
 Proof.
@@ -402,7 +410,7 @@ Qed.
 
 Lemma int_typed_spec_alt x τ :
   int_typed x τ ↔
-    match ISign τ with
+    match sign τ with
     | Signed => -2 ^ int_bits τ ≤ 2 * x < 2 ^ int_bits τ
     | Unsigned => 0 ≤ x < 2 ^ int_bits τ
     end.
@@ -414,7 +422,7 @@ Proof.
 Qed.
 Lemma int_typed_nonneg_signed x τ :
   0 ≤ 2 * x < 2 ^ int_bits τ → int_typed x τ.
-Proof. rewrite int_typed_spec_alt. destruct (ISign _); lia. Qed.
+Proof. rewrite int_typed_spec_alt. destruct (sign _); lia. Qed.
 Lemma int_typed_small x τ : 0 ≤ x < 128 → int_typed x τ.
 Proof.
   intros [??]. apply int_typed_nonneg_signed. split; [lia|].
@@ -430,8 +438,8 @@ Lemma int_to_of_bits τ bs :
   length bs = int_bits τ → int_to_bits τ (int_of_bits τ bs) = bs.
 Proof.
   intros Hlen. unfold int_to_bits, int_of_bits.
-  rewrite <-!Hlen, <-!(deendianize_length (IRank τ) bs); clear Hlen.
-  pose proof (Z_of_bits_range (deendianize (IRank τ) bs)).
+  rewrite <-!Hlen, <-!(deendianize_length (rank τ) bs); clear Hlen.
+  pose proof (Z_of_bits_range (deendianize (rank τ) bs)).
   destruct τ as [[] k]; simpl in *.
   * repeat case_decide; auto with lia.
     + by rewrite Z_to_of_bits, endianize_deendianize.
@@ -446,13 +454,12 @@ Proof.
   intros. rewrite <-(int_to_of_bits τ bs1),
     <-(int_to_of_bits τ bs2) by done; congruence.
 Qed.
-
 Lemma int_of_bits_typed τ bs :
   length bs = int_bits τ → int_typed (int_of_bits τ bs) τ.
 Proof.
   intros Hlen. unfold int_of_bits. generalize (int_bits_pos τ).
-  generalize (Z_of_bits_range (deendianize (IRank τ) bs)).
-  rewrite int_typed_spec_alt, <-!Hlen, <-!(deendianize_length (IRank τ) bs).
+  generalize (Z_of_bits_range (deendianize (rank τ) bs)).
+  rewrite int_typed_spec_alt, <-!Hlen, <-!(deendianize_length (rank τ) bs).
   destruct τ as [[] k]; simpl; repeat case_decide; auto with lia.
 Qed.
 Lemma int_of_to_bits τ x : int_typed x τ → int_of_bits τ (int_to_bits τ x) = x.
@@ -464,13 +471,12 @@ Proof.
       rewrite deendianize_endianize, Z_of_to_bits; lia.
   * intros [??]. by rewrite deendianize_endianize, Z_of_to_bits.
 Qed.
-
 Lemma int_of_zero_bits τ : int_of_bits τ (replicate (int_bits τ) false) = 0.
 Proof.
   assert (∀ k n b, deendianize k (replicate n b) = replicate n b) as Hrepl.
   { intros k n b. symmetry. apply replicate_Permutation.
     by rewrite deendianize_permutation. }
-  unfold int_of_bits. destruct (ISign τ).
+  unfold int_of_bits. destruct (sign τ).
   * case_decide as Hbs; [by rewrite Hrepl, Z_of_zero_bits |].
     destruct Hbs. rewrite Hrepl, Z_of_zero_bits, Z.mul_0_r. auto with zpos.
   * by rewrite Hrepl, Z_of_zero_bits.
@@ -479,18 +485,34 @@ Lemma int_to_bits_signed_unsigned k x :
   0 ≤ x → int_to_bits (IntType Signed k) x = int_to_bits (IntType Unsigned k) x.
 Proof. unfold int_to_bits; simpl; case_decide; auto with lia. Qed.
 
-Lemma int_binop_ok_typed_ τ op x y :
+Lemma int_pre_arithop_typed op x y τ :
   int_typed x τ → int_typed y τ →
-  int_binop_ok_ τ op x y → int_typed (int_binop_ τ op x y) τ.
+  int_pre_arithop_ok op x y τ → int_typed (int_pre_arithop op x y τ) τ.
 Proof.
-  unfold int_typed, int_binop_ok_, int_binop_. intros [??] [??]. destruct op.
-  * destruct (ISign τ); auto with lia.
-  * destruct (ISign τ); auto with lia.
-  * destruct (ISign τ); auto with lia.
-  * destruct (ISign τ); auto with lia. intros (?&[? _]&?). split; auto.
+  unfold int_typed, int_pre_arithop_ok, int_pre_arithop.
+  intros [??] [??]. destruct op.
+  * destruct (sign τ); auto with lia.
+  * destruct (sign τ); auto with lia.
+  * destruct (sign τ); auto with lia.
+  * intros Hy. unfold int_lower, int_upper in *. destruct (sign τ); [lia|].
+    apply Z_quot_range_nonneg; auto with lia.
+  * intros Hy. unfold int_lower, int_upper in *. destruct (sign τ).
+    + generalize (Z.rem_bound_abs x y Hy). destruct (decide (0 < y)).
+      - rewrite (Z.abs_eq y), Z.abs_lt by lia. lia.
+      - rewrite (Z.abs_neq y), Z.abs_lt by lia. lia.
+    + split; [apply Z.rem_bound_pos; lia|].
+      transitivity y; auto. apply Z.rem_bound_pos; lia.
+Qed.
+Lemma int_pre_shiftop_typed op x y τ τ2 :
+  int_typed x τ → int_typed y τ2 →
+  int_pre_shiftop_ok op x y τ → int_typed (int_pre_shiftop op x y τ) τ.
+Proof.
+  unfold int_typed, int_pre_shiftop_ok, int_pre_shiftop.
+  intros [??] [??]. destruct op.
+  * destruct (sign τ); auto with lia. intros (?&[? _]&?). split; auto.
     rewrite Z.shiftl_mul_pow2 by done. transitivity 0; auto with zpos.
   * intros ?. assert (0 ≤ x ∧ 0 ≤ y) as [??].
-    { unfold int_lower, int_upper in *. destruct (ISign τ); auto with lia. }
+    { unfold int_lower, int_upper in *. destruct (sign τ); auto with lia. }
     rewrite Z.shiftr_div_pow2 by done. split.
     + transitivity 0; auto. apply Z.div_pos; auto with zpos.
     + apply Z.le_lt_trans with x; auto.
@@ -498,33 +520,105 @@ Proof.
       transitivity (1 * x); auto with lia.
       apply Z.mul_le_mono_nonneg_r; auto with zpos.
       assert (0 < 2 ^ y); auto with zpos.
-  * intros Hy. unfold int_lower, int_upper in *. destruct (ISign τ); [lia|].
-    apply Z_quot_range_nonneg; auto with lia.
-  * intros Hy. unfold int_lower, int_upper in *. destruct (ISign τ).
-    + generalize (Z.rem_bound_abs x y Hy). destruct (decide (0 < y)).
-      - rewrite (Z.abs_eq y), Z.abs_lt by lia. lia.
-      - rewrite (Z.abs_neq y), Z.abs_lt by lia. lia.
-    + split; [apply Z.rem_bound_pos; lia|].
-      transitivity y; auto. apply Z.rem_bound_pos; lia.
-  * intros _. by case_decide; apply int_typed_small.
-  * intros ?. apply int_of_bits_typed.
-    rewrite zip_with_length, !int_to_bits_length; lia.
 Qed.
-Lemma int_cast_ok_typed_ σ x :
-  int_cast_ok_ σ x → int_typed (int_cast_ σ x) σ.
+Lemma int_pre_cast_typed x σ :
+  int_pre_cast_ok σ x → int_typed (int_pre_cast σ x) σ.
 Proof.
-  unfold int_typed, int_cast_ok_, int_cast_. destruct (ISign σ); auto with lia.
+  unfold int_typed, int_pre_cast_ok, int_pre_cast.
+  destruct (sign σ); auto with lia.
 Qed.
-End int_coding.
-
-Section int_env.
-Context `{IntEnvSpec Ti}.
-
-Lemma int_unop_ok_typed op x τ :
-  int_typed x τ → int_unop_ok τ op x → int_typed (int_unop τ op x) τ.
+Lemma int_typed_pre_cast_ok x σ : int_typed x σ → int_pre_cast_ok σ x.
+Proof. unfold int_pre_cast_ok. by destruct (sign σ). Qed.
+Lemma int_typed_pre_cast x σ : int_typed x σ → int_pre_cast σ x = x.
 Proof.
-  destruct op; simpl.
-  * intros. apply int_binop_ok_typed; auto. by apply int_typed_small.
-  * intros. apply int_of_bits_typed. by rewrite fmap_length, int_to_bits_length.
+  unfold int_pre_cast, int_typed, int_lower, int_upper.
+  destruct (sign σ); auto using Z.mod_small.
 Qed.
-End int_env.
+Lemma int_unsigned_pre_cast_ok x σ : sign σ = Unsigned → int_pre_cast_ok σ x.
+Proof. unfold int_pre_cast_ok. by intros ->. Qed.
+
+Lemma int_rank_bits_le τ σ :
+  rank_size (rank τ) ≤ rank_size (rank σ) → int_bits τ ≤ int_bits σ.
+Proof.
+  intros. unfold int_bits. rewrite !Nat2Z.inj_mul.
+  apply Z.mul_le_mono_nonneg_r; lia.
+Qed.
+Lemma int_rank_bits_lt τ σ :
+  rank_size (rank τ) < rank_size (rank σ) → int_bits τ < int_bits σ.
+Proof.
+  intros. unfold int_bits. rewrite !Nat2Z.inj_mul.
+  apply Z.mul_lt_mono_pos_r; auto. apply (Nat2Z.inj_lt 0), char_bits_pos.
+Qed.
+Lemma int_typed_rank_le x τ σ :
+  sign τ = sign σ → rank_size (rank τ) ≤ rank_size (rank σ) →
+  int_typed x τ → int_typed x σ.
+Proof.
+  rewrite !int_typed_spec_alt; intros <-; destruct (sign τ).
+  * intros ? [??]; split.
+    + transitivity (- 2 ^ int_bits τ); [|done]. rewrite <-Z.opp_le_mono.
+      by apply Z.pow_le_mono_r; auto using int_rank_bits_le.
+    + apply Z.lt_le_trans with (2 ^ int_bits τ); [done|].
+      by apply Z.pow_le_mono_r; auto using int_rank_bits_le.
+  * intros ? [??]; split; [done|].
+    apply Z.lt_le_trans with (2 ^ int_bits τ); [done|].
+    by apply Z.pow_le_mono_r; auto using int_rank_bits_le.
+Qed.
+Lemma int_typed_rank_lt x τ σ :
+  sign τ = Unsigned → rank_size (rank τ) < rank_size (rank σ) →
+  int_typed x τ → int_typed x σ.
+Proof.
+  destruct (decide (sign σ = sign τ));[eauto using int_typed_rank_le with lia|].
+  rewrite !int_typed_spec_alt. destruct (sign σ); [|congruence].
+  intros -> ? [??]; split.
+  * transitivity (-0); [|lia]. rewrite <-Z.opp_le_mono. by apply Z.pow_nonneg.
+  * rewrite <-Z_pow_pred_r, <-Z.mul_lt_mono_pos_l by (by auto).
+    apply Z.lt_le_trans with (2 ^ int_bits τ); [done|].
+    by apply Z.pow_le_mono_r, Z.lt_le_pred; auto using int_rank_bits_lt.
+Qed.
+
+Local Arguments int_promote _ _ !_ /.
+Local Arguments union _ _ !_ !_ /.
+Local Arguments int_union _ _ !_ !_ /.
+Lemma int_promote_promote σ : int_promote (int_promote σ) = int_promote σ.
+Proof. destruct σ; simplify_option_equality; congruence. Qed.
+Lemma int_promote_typed x σ : int_typed x σ → int_typed x (int_promote σ).
+Proof.
+  destruct σ as [[] k]; simpl in *; repeat case_decide; auto.
+  * apply int_typed_rank_le; simpl; auto with lia.
+  * by replace k with int_rank by (by apply (injective rank_size)).
+  * by apply int_typed_rank_lt.
+  * apply int_typed_rank_le; simpl; auto with lia.
+Qed.
+Global Instance: Commutative (=) (@union (int_type Ti) _).
+Proof.
+  intros [s1 k1] [s2 k2]; simpl.
+  repeat case_decide; intuition; simplify_equality'; try lia.
+  * f_equal; apply (injective rank_size); lia.
+  * destruct s1, s2; intuition lia.
+Qed.
+Global Instance: Associative (=) (@union (int_type Ti) _).
+Proof.
+  intros [[] ?] [[] ?] [[] ?]; repeat
+    match goal with
+    | _ => reflexivity
+    | H : _ ∧ _ |- _ => destruct H
+    | _ => progress simplify_equality'
+    | _ => repeat case_decide
+    end; intuition lia.
+Qed.
+Global Instance: Idempotent (=) (@union (int_type Ti) _).
+Proof. by intros [s k]; simplify_option_equality. Qed.
+Lemma int_union_pre_cast_ok_l x τ1 τ2 :
+  int_typed x τ1 → int_pre_cast_ok (τ1 ∪ τ2) x.
+Proof.
+  unfold union, int_union; repeat case_decide;
+    eauto using int_typed_pre_cast_ok, int_typed_rank_le.
+  { intuition eauto using int_unsigned_pre_cast_ok. }
+  assert (sign τ1 = Unsigned ∧ rank_size (rank τ1) < rank_size (rank τ2)) as [].
+  { destruct (sign τ1), (sign τ2); intuition lia. }
+  eauto using int_typed_pre_cast_ok, int_typed_rank_lt.
+Qed.
+Lemma int_union_pre_cast_ok_r x τ1 τ2 :
+  int_typed x τ1 → int_pre_cast_ok (τ2 ∪ τ1) x.
+Proof. intros. rewrite (commutative (∪)). by apply int_union_pre_cast_ok_l. Qed.
+End properties.
